src/fs/dir/dirent.dfy
@@ -33,7 +33,7 @@ module DirEntries
     ensures path_len == dirent_sz - 8
   {}
 
-  predicate {:opaque} is_pathc(s: String)
+  ghost predicate {:opaque} is_pathc(s: String)
   {
     && |s| <= MAX_FILENAME_SZ as nat
     && forall i | 0 <= i < |s| :: s[i] != 0
@@ -41,20 +41,20 @@ module DirEntries
 
   type PathComp = s:String | is_pathc(s) ghost witness (reveal is_pathc(); [])
 
-  function method empty_path(): PathComp
+  function empty_path(): PathComp
   {
     reveal is_pathc();
     []
   }
 
-  function method encode_pathc(pc: PathComp): (s:seq<byte>)
+  function encode_pathc(pc: PathComp): (s:seq<byte>)
     ensures |s| == path_len
   {
     reveal is_pathc();
     pc + C.repeat(0 as byte, path_len - |pc|)
   }
 
-  function method decode_null_terminated(s: seq<byte>): String
+  function decode_null_terminated(s: seq<byte>): String
   {
     if s == [] then []
     else
@@ -68,7 +68,7 @@ module DirEntries
     ensures forall i | 0 <= i < |decode_null_terminated(s)| :: decode_null_terminated(s)[i] != 0
   {}
 
-  function method decode_pathc(s: seq<byte>): PathComp
+  function decode_pathc(s: seq<byte>): PathComp
     requires |s| == path_len
   {
     decode_null_terminated_spec(s);
@@ -127,19 +127,19 @@ module DirEntries
 
     // we don't call this valid because unused DirEnts do show up (eg, a Dirents
     // will in general have unused DirEnts and this isn't a problem)
-    predicate method used()
+    predicate used()
     {
       ino != 0
     }
 
     static predicate method is_used(e: DirEnt) { e.used() }
 
-    predicate method unused()
+    predicate unused()
     {
       ino == 0
     }
 
-    function {:opaque} encoding(): seq<Encodable>
+    ghost function {:opaque} encoding(): seq<Encodable>
     {
       [EncBytes(encode_pathc(name)), EncUInt64(ino)]
     }
@@ -149,7 +149,7 @@ module DirEntries
     //
     // this function doesn't really show up often anyway so it probably won't
     // trigger too many things
-    function enc(): seq<byte>
+    ghost function enc(): seq<byte>
     {
       Marshal.seq_encode(encoding())
     }
@@ -178,7 +178,7 @@ module DirEntries
 
   type Directory = map<PathComp, Ino>
 
-  function seq_to_dir(s: seq<DirEnt>): Directory
+  ghost function seq_to_dir(s: seq<DirEnt>): Directory
   {
     if s == [] then map[]
     else (
@@ -190,7 +190,7 @@ module DirEntries
       )
   }
 
-  function method used_dirents(s: seq<DirEnt>): seq<DirEnt>
+  function used_dirents(s: seq<DirEnt>): seq<DirEnt>
   {
     C.seq_filter(DirEnt.is_used, s)
   }
@@ -264,7 +264,7 @@ module DirEntries
     // }
   }
 
-  predicate {:opaque} dirents_unique(s: seq<DirEnt>)
+  ghost predicate {:opaque} dirents_unique(s: seq<DirEnt>)
   {
     forall i, j | 0 <= i < |s| && 0 <= j < |s| ::
       s[i].name == s[j].name && s[i].used() && s[j].used() ==> i == j
@@ -406,7 +406,7 @@ module DirEntries
       zeros_dir(64);
     }
 
-    predicate Valid()
+    ghost predicate Valid()
     {
       // 128*32 == 4096 so these will fit in a block
       && |s| <= dir_sz
@@ -423,7 +423,7 @@ module DirEntries
     // note that this does not require Valid, so we can call it on a Dirents(s)
     // without first proving validity (that is, it's really a method for any
     // seq<DirEnt>)
-    function {:opaque} enc(): (data:seq<byte>)
+    ghost function {:opaque} enc(): (data:seq<byte>)
       ensures |data| == dirent_sz*|s|
     {
       C.concat_homogeneous_len(C.seq_fmap(encOne, this.s), dirent_sz);
@@ -453,7 +453,7 @@ module DirEntries
       zeros_enc(64);
     }
 
-    function insert_ent(i: nat, e: DirEnt): (ents': Dirents)
+    ghost function insert_ent(i: nat, e: DirEnt): (ents': Dirents)
       requires Valid()
       requires i < |s|
       requires this.findName(e.name) >= |s|
@@ -482,7 +482,7 @@ module DirEntries
       (e:DirEnt) => e.used() && e.name == p
     }
 
-    function findName(p: PathComp): (i:nat)
+    ghost function findName(p: PathComp): (i:nat)
       requires Valid()
     {
       C.find_first(findName_pred(p), s)
@@ -518,7 +518,7 @@ module DirEntries
       }
     }
 
-    predicate {:opaque} find_free_spec(i: nat)
+    ghost predicate {:opaque} find_free_spec(i: nat)
     {
       && i <= |s|
       && forall k:nat | k < i :: s[k].used()
@@ -529,7 +529,7 @@ module DirEntries
       !e.used()
     }
 
-    function method findFree(): (i:nat)
+    function findFree(): (i:nat)
       requires Valid()
       ensures i < |s| ==> !s[i].used()
       ensures find_free_spec(i)
@@ -570,7 +570,7 @@ module DirEntries
       zeros_enc(n);
     }
 
-    function {:opaque} extend_zero(n: nat): (dents: Dirents)
+    ghost function {:opaque} extend_zero(n: nat): (dents: Dirents)
       requires Valid()
       requires |s| + n <= dir_sz
       ensures dents.Valid()
