src/fs/inode/mem_inode.dfy
@@ -19,7 +19,7 @@ module MemInodes {
     ghost const Repr: set<object> := {this, bs}
 
     // the inode represented
-    function val(): Inode.Inode
+    ghost function val(): Inode.Inode
       reads Repr
       requires Valid()
     {
@@ -27,13 +27,13 @@ module MemInodes {
       Inode.Mk(Inode.Meta(sz, attrs), blks)
     }
 
-    function method ty(): Inode.InodeType
+    function ty(): Inode.InodeType
       reads this
     {
       attrs.ty
     }
 
-    predicate {:opaque} Valid()
+    ghost predicate {:opaque} Valid()
       reads Repr
     {
       && |blks| == 12
@@ -42,7 +42,7 @@ module MemInodes {
       && Marshal.decode_uint64_seq(bs.data[32..]) == blks
     }
 
-    function method meta(): Inode.Meta
+    function meta(): Inode.Meta
       reads this
     {
       Inode.Meta(sz, attrs)
