src/machine/machine.dfy
@@ -10,12 +10,12 @@ module Machine {
     newtype {:nativeType "uint"} uint32 = x:int | 0 <= x < U32.MAX
     newtype {:nativeType "ulong"} uint64 = x:int | 0 <= x < U64.MAX
 
-    predicate no_overflow(x: nat, y: int)
+    ghost predicate no_overflow(x: nat, y: int)
     {
         0 <= x + y < U64.MAX
     }
 
-    function method sum_overflows(x: uint64, y: uint64): (overflow:bool)
+    function sum_overflows(x: uint64, y: uint64): (overflow:bool)
         ensures !overflow == no_overflow(x as nat, y as nat)
     {
         // discovered by trial and error
@@ -26,12 +26,12 @@ module Machine {
     // modules into their parents but not the other way around, so there's no
     // way to do that without making U64 a separate module (which I don't know
     // how to re-export)
-    predicate no_overflow_u64(x: uint64, y: int)
+    ghost predicate no_overflow_u64(x: uint64, y: int)
     {
         no_overflow(x as nat, y)
     }
 
-    function method min_u64(x: uint64, y: uint64): uint64
+    function min_u64(x: uint64, y: uint64): uint64
     {
         if x < y then x else y
     }
@@ -40,7 +40,7 @@ module Machine {
         ensures min_u64(x, y) <= x && min_u64(x, y) <= y
     {}
 
-    function method max_u64(x: uint64, y: uint64): uint64
+    function max_u64(x: uint64, y: uint64): uint64
     {
         if x > y then x else y
     }
