src/util/lock_order.dfy
@@ -8,18 +8,18 @@ module LockOrder {
 
   const EmptyLockHint: LockHint := []
 
-  function method has_lock(locks: LockHint, h: uint64): bool
+  function has_lock(locks: LockHint, h: uint64): bool
   {
     h in locks
   }
 
   // is it safe to acquire l, with locks held?
-  function method safe_lock(locks: LockHint, l: uint64): bool
+  function safe_lock(locks: LockHint, l: uint64): bool
   {
     locks == [] || has_lock(locks, l) || l > locks[|locks|-1]
   }
 
-  function method insert_lock_hint(locks: LockHint, h: uint64): LockHint
+  function insert_lock_hint(locks: LockHint, h: uint64): LockHint
   {
     if locks == [] then [h]
     else if h < locks[0] then [h] + locks
@@ -27,14 +27,14 @@ module LockOrder {
     else [locks[0]] + insert_lock_hint(locks[1..], h)
   }
 
-  function method insert_lock_hints(locks: LockHint, hs: seq<uint64>): LockHint
+  function insert_lock_hints(locks: LockHint, hs: seq<uint64>): LockHint
     decreases |hs|
   {
     if hs == [] then locks
     else insert_lock_hints(insert_lock_hint(locks, hs[0]), hs[1..])
   }
 
-  predicate lock_hints_sorted(locks: LockHint)
+  ghost predicate lock_hints_sorted(locks: LockHint)
   {
     forall i, j | 0 <= i < j < |locks| :: locks[i] <= locks[j]
   }
