src/util/std.dfy
@@ -2,13 +2,13 @@ module Std
 {
   datatype Option<T> = Some(x:T) | None
   {
-    function method get_default(def: T): T
+    function get_default(def: T): T
     {
       if Some? then x else def
     }
   }
 
-  function map_delete<K, V>(m: map<K, V>, k0: K): map<K, V>
+  ghost function map_delete<K, V>(m: map<K, V>, k0: K): map<K, V>
   {
     map k: K | k in m && k != k0 :: m[k]
   }
